Fifo proofs2 (#64)
* Changes to implementation and fix of spec, also (size = 1) proof
for fifo impl/spec.

* Invariant is correct, changes needed to EclecticLib.

* Moving generic lemms from RegArray to Kami.

* Qed of Fifo (Spec) <= FifoList. Requires Kami update.

Fifo/Proofs.v
@@ -7,7 +7,7 @@ Require Import Kami.GallinaModules.Relations.
 Require Import Kami.GallinaModules.AuxLemmas.
 Require Import Kami.GallinaModules.AuxTactics.
 Require Import StdLibKami.RegArray.Proofs.
-  
+
 Record FifoCorrect {FParams} (imp spec : @Fifo.Ifc.Ifc FParams) : Type :=
   {
     fifoRegs : list (Attribute FullKind);
@@ -162,3 +162,539 @@ Section Proofs2.
   Qed.
   
 End Proofs2.
+
+Section Proofs3.
+  
+  Context {ifcParams' : Fifo.Ifc.Params}.
+  (* Context {raIfcParams' : RegArray.Ifc.Params}. *)
+  
+  Variable pow2 : Nat.pow 2 (Nat.log2_up size) = size.
+  Local Definition implParams : Fifo.Impl.Params := 
+    {|Impl.sizePow2 :=  pow2
+      ; Impl.regArray := RegArray.Spec.spec|}.
+  
+  Local Definition fifoImpl := @Fifo.Impl.impl ifcParams' implParams.
+  Local Definition fifoSpec := @Fifo.Spec.spec ifcParams'.
+
+  Section Size1.
+    Variable Hsize1 : size = 1.
+
+    Record myFifoR  (o_i o_s : RegsT) : Prop :=
+      {
+        implRegs : RegsT;
+        specRegs : RegsT;
+        fifo1_bval : bool;
+        fifo1_dval : type k;
+        implRegVal : implRegs = [(Fifo1.validRegName,
+                                  existT _ (SyntaxKind Bool) fifo1_bval);
+                                (Fifo1.dataRegName,
+                                 existT _ (SyntaxKind k) fifo1_dval)];
+        specRegVal : specRegs = [(Spec.listName,
+                                  existT (fullType type) (Spec.nlist type) (if fifo1_bval
+                                                                            then [fifo1_dval]
+                                                                            else nil))];
+        Ho_iCorrect1 : o_i = implRegs;
+        Ho_sCorrect1 : o_s = specRegs;
+        Ho_iNoDup1' : NoDup (map fst o_i);
+      }.
+
+    Ltac Record_destruct :=
+      match goal with
+      |[ H : myFifoR _ _ |- _] => destruct H
+      end.
+    
+    Goal FifoCorrect fifoImpl fifoSpec.
+      rewrite <- Nat.eqb_eq in Hsize1.
+      all : econstructor 1 with (fifoR := myFifoR)
+                                (fifoRegs := [(Fifo1.validRegName,
+                                               SyntaxKind Bool);
+                                              (Fifo1.dataRegName,
+                                               SyntaxKind k)]).
+      all : red; unfold fifoImpl, fifoSpec, impl, spec, regArray,
+                 isEmpty, flush, enq, deq, numFree, isFull, first,
+                 Impl.isEmpty, Impl.flush, Impl.enq, Impl.deq, Impl.numFree,
+                 Impl.isFull, Impl.first,
+                 Spec.isEmpty, Spec.flush, Spec.enq, Spec.deq, Spec.numFree,
+                 Spec.isFull, Spec.first.
+      all : try rewrite Hsize1; unfold Fifo1.impl, Fifo1.isEmpty,
+                                Fifo1.isFull, Fifo1.flush, Fifo1.numFree, Fifo1.first,
+                                Fifo1.deq, Fifo1.enq; intros; try Record_destruct.
+      all : rewrite Nat.eqb_eq in Hsize1.
+      - hyp_consumer; goal_consumer1.
+        destruct x; auto.
+      - hyp_consumer; goal_consumer2; eauto.
+      - hyp_consumer; goal_consumer1.
+        destruct x; simpl; symmetry.
+        + rewrite negb_true_iff, Nat.ltb_ge.
+          lia.
+        + rewrite negb_false_iff, Nat.ltb_lt.
+          lia.
+      - hyp_consumer; goal_consumer2; eauto.
+      - hyp_consumer; goal_consumer1.
+        destruct x; simpl; rewrite Hsize1; arithmetizeWord; auto.
+      - hyp_consumer; goal_consumer2; eauto.
+      - hyp_consumer; goal_consumer1.
+        destruct x; cbn[Spec.getHead emptyb negb]; apply functional_extensionality_dep;
+          intros; fin_dep_destruct x; auto; fin_dep_destruct y; auto.
+      - hyp_consumer; goal_consumer2.
+      - hyp_consumer; goal_consumer1.
+        +  destruct x; cbn[Spec.getHead emptyb negb]; apply functional_extensionality_dep;
+             intros; fin_dep_destruct x; auto; fin_dep_destruct y; auto.
+        + econstructor; eauto; normalize_key_concl.
+          destruct x; simpl; auto.
+      - hyp_consumer; goal_consumer2.
+      - hyp_consumer; goal_consumer1.
+        + destruct x; simpl; symmetry.
+          * rewrite Nat.ltb_ge; lia.
+          * rewrite Nat.ltb_lt; lia.
+        + econstructor; eauto; normalize_key_concl.
+          destruct x; cbv[Spec.snocInBound]; rewrite Hsize1; simpl; reflexivity.
+      - hyp_consumer; goal_consumer2.
+      - hyp_consumer; goal_consumer1.
+        econstructor; eauto; normalize_key_concl.
+    Qed.
+  
+  End Size1.
+
+  Section SizeGT1.
+    Variable Hsize1 : size <> 1.
+    Definition listInSpec (len start : nat) (arr : Fin.t size -> type k) :=
+      firstn len (rotateList start (convertToList arr)).
+
+    Record myFifoSpecR (o_i o_s : RegsT) : Prop :=
+    {   
+      implRegs : RegsT;
+      specRegs : RegsT;
+      regArray : RegsT;
+      queueLen : Z;
+      enqVal : word (Fifo.Ifc.lgSize + 1);
+      deqVal : word (Fifo.Ifc.lgSize + 1);
+      arrayVal : Fin.t size -> type k;
+      HqueueLen : queueLen = wordVal _ (enqVal ^- deqVal);
+      Hbound : (queueLen <= Z.of_nat size)%Z;
+      implRegVal : implRegs = [(Fifo.Impl.deqPtrName,
+                                existT _ (SyntaxKind (Bit (Fifo.Ifc.lgSize + 1))) deqVal);
+                              (Fifo.Impl.enqPtrName,
+                               existT _ (SyntaxKind (Bit (Fifo.Ifc.lgSize + 1))) enqVal)];
+      regArrayVal : regArray = [((name ++ ".regArray")%string,
+                                  existT _ (SyntaxKind (Array size k)) arrayVal)];
+      specRegVal : specRegs = [(Spec.listName,
+                                     existT (fullType type) (Fifo.Spec.nlist type)
+                                            (listInSpec (Z.to_nat queueLen)
+                                                        (Z.to_nat ((wordVal _ deqVal)
+                                                         mod (2 ^ Z.of_nat (Nat.log2_up size))))
+                                                        arrayVal))];
+      Ho_iCorrect : o_i = implRegs ++ regArray;
+      Ho_sCorrect : o_s = specRegs;
+      Ho_iNoDup' : NoDup (map fst o_i);
+    }.
+
+    Ltac Record_destruct :=
+      match goal with
+      |[ H : myFifoSpecR _ _ |- _] => destruct H
+      end.
+    
+    Goal FifoCorrect fifoImpl fifoSpec.
+      assert (size <> 0) as P.
+      { destruct size; auto. }
+      assert (2 ^ (lgSize + 1) <> 0) as P0.
+      { unfold lgSize; intro P0.
+        rewrite Nat.pow_add_r, pow2 in P0.
+        destruct size; simpl in pow2; try lia.
+        simpl in P0; lia.
+      }
+      rewrite <- Nat.eqb_neq in Hsize1.
+      all : econstructor 1 with (fifoR := myFifoSpecR)
+                                (fifoRegs := [(Fifo.Impl.deqPtrName,
+                                               SyntaxKind (Bit (Fifo.Ifc.lgSize + 1)));
+                                              (Fifo.Impl.enqPtrName,
+                                               SyntaxKind (Bit (Fifo.Ifc.lgSize + 1)));
+                                              (Spec.arrayName,
+                                               (SyntaxKind (Array size k)))]).
+      all : red; unfold fifoImpl, fifoSpec, impl, spec, regArray,
+                 isEmpty, flush, enq, deq, numFree, isFull, first,
+                 Impl.isEmpty, Impl.flush, Impl.enq, Impl.deq, Impl.numFree,
+                 Impl.isFull, Impl.first,
+                 Spec.isEmpty, Spec.flush, Spec.enq, Spec.deq, Spec.numFree,
+                 Spec.isFull, Spec.first.
+      all : try rewrite Hsize1; rewrite Nat.eqb_neq in Hsize1.
+      all : unfold Ifc.read, Ifc.write, regArray, implParams, Spec.spec, Spec.read, Spec.write,
+        Impl.isEmpty, Ifc.size, Ifc.k; intros; try Record_destruct.
+      - hyp_consumer.
+        goal_consumer1; simpl.
+        destruct weq; subst; simpl; symmetry; unfold listInSpec.
+        + rewrite Z.sub_diag, Zmod_0_l, firstn_O; reflexivity.
+        + rewrite emptyb_false_len, firstn_length_le;
+            [|simpl in *; rewrite rotateLength, <- list_arr_length; lia].
+          specialize (Nat.le_0_l
+                        (Z.to_nat ((wordVal (lgSize + 1) x1
+                                    - wordVal (lgSize + 1) x) mod 2 ^ Z.of_nat (lgSize + 1))))
+            as P1.
+          destruct (le_lt_or_eq _ _ P1); auto.
+          exfalso.
+          apply neq_wordVal in n; apply n.
+          specialize (wordBound _ x) as P2; specialize (wordBound _ x1) as P3.
+          rewrite boundProofZIff in *.
+          simpl in Hbound.
+          symmetry in H0.
+          assert (0 = Z.to_nat 0) as TMP by lia; rewrite TMP in H0; clear TMP.
+          apply Z2Nat.inj in H0; try lia; [|apply Z.mod_pos_bound; lia].
+          apply Znumtheory.Zmod_divide_minus in H0; try lia.
+          rewrite Z.sub_0_r in H0; unfold Z.divide in H0; dest.
+          unfold lgSize in *.
+          rewrite <- Zpow_of_nat, Nat.pow_add_r, pow2, Nat2Z.inj_mul in *; simpl in *.
+          destruct (Z_dec 0 x0) as [[P2 | P2] | P2]; try lia.
+          * apply Zlt_le_succ in P2; simpl in P2; try lia.
+            apply (Z.mul_le_mono_nonneg_r _ _ (Z.of_nat size * 2)) in P2; lia.
+          * apply Z.gt_lt in P2.
+            rewrite Z.lt_le_pred in P2; simpl in P2.
+            apply (Z.mul_le_mono_nonneg_r _ _ (Z.of_nat size * 2)) in P2; lia.
+      - hyp_consumer.
+        goal_consumer2; eauto.
+      - hyp_consumer.
+        goal_consumer1; simpl.
+        destruct weq; simpl; symmetry; unfold listInSpec.
+        + rewrite negb_true_iff, Nat.ltb_ge, firstn_length_le;
+            [|simpl in *; rewrite rotateLength, <- list_arr_length; lia].
+          destruct (Zle_lt_or_eq _ _ Hbound); simpl in *; try lia.
+          exfalso; rewrite <- e in H0; simpl in H0.
+          rewrite Zplus_mod_idemp_r, Zplus_mod_idemp_l,
+          Zminus_mod_idemp_l, Z.add_simpl_l, Z.mod_small in H0; try lia.
+          unfold lgSize in *.
+          rewrite <- Zpow_of_nat, Nat.pow_add_r, pow2, Nat2Z.inj_mul in *; simpl in *; lia.
+        + rewrite negb_false_iff, Nat.ltb_lt, firstn_length_le;
+            [|simpl in *; rewrite rotateLength, <- list_arr_length; lia].
+          destruct (Zle_lt_or_eq _ _ Hbound); simpl in *; try lia.
+          exfalso.
+          apply neq_wordVal in n; apply n; simpl.
+          rewrite <- H0, Zplus_mod_idemp_l.
+          repeat rewrite Zplus_mod_idemp_r.
+          rewrite Zplus_minus, (wordBound _ x1); reflexivity.
+      - hyp_consumer.
+        goal_consumer2; eauto.
+      - hyp_consumer.
+        goal_consumer1; simpl; unfold listInSpec; rewrite firstn_length_le;
+          [|simpl in *; rewrite rotateLength, <- list_arr_length; lia].
+        arithmetizeWord; destruct x, x1; simpl in *.
+        rewrite Zminus_mod_idemp_l.
+        rewrite (Z.mod_small
+                   (Z.of_nat size - (wordVal0 - wordVal) mod 2 ^ Z.of_nat (lgSize + 1))
+                   (2 ^ Z.of_nat (lgSize + 1))).
+        + rewrite Nat2Z.inj_sub, Z2Nat.id; try lia.
+          apply Z.mod_pos_bound.
+          unfold lgSize in *.
+          rewrite <- Zpow_of_nat, Nat.pow_add_r, pow2, Nat2Z.inj_mul in *; simpl in *; lia.
+        + unfold lgSize in *.
+          rewrite <- Zpow_of_nat, Nat.pow_add_r, pow2, Nat2Z.inj_mul in *; simpl in *; try lia.
+          specialize (Z.mod_pos_bound (wordVal0 - wordVal) (Z.of_nat size * 2) ltac:(lia)) as P1;
+            lia.
+      - hyp_consumer.
+        goal_consumer2; eauto.
+      - hyp_consumer.
+        goal_consumer1.
+        apply functional_extensionality_dep.
+        intros; fin_dep_destruct x.
+        + simpl; destruct weq; subst; simpl; symmetry; unfold listInSpec.
+          * rewrite negb_false_iff, Z.sub_diag, Zmod_0_l, firstn_O; reflexivity.
+          * rewrite negb_true_iff, emptyb_false_len, firstn_length_le;
+              [|simpl in *; rewrite rotateLength, <- list_arr_length; lia].
+            specialize (Nat.le_0_l
+                          (Z.to_nat ((wordVal (lgSize + 1) x10
+                                     - wordVal (lgSize + 1) x6)
+                                       mod 2 ^ Z.of_nat (lgSize + 1)))) as P1.
+            destruct (le_lt_or_eq _ _ P1); auto.
+            exfalso.
+            specialize (wordBound _ x6) as P2; specialize (wordBound _ x10) as P3.
+            rewrite boundProofZIff in *.
+            apply neq_wordVal in n; apply n.
+            unfold lgSize in *.
+            rewrite <- Zpow_of_nat, Nat.pow_add_r, pow2, Nat2Z.inj_mul in *; simpl in *; try lia.
+            assert (0 = Z.to_nat 0) as TMP by auto; rewrite TMP in H1 at 1; clear TMP.
+            apply Z2Nat.inj in H1; [|lia |apply Z.mod_pos_bound; lia ].
+            symmetry in H1.
+            apply Z.mod_divide in H1; try lia; unfold Z.divide in H1; dest.
+            destruct (Z_dec 0 x) as [[P2 | P2] | P2]; try lia.
+            -- apply Zlt_le_succ in P2; simpl in P2; try lia.
+               apply (Z.mul_le_mono_nonneg_r _ _ (Z.of_nat size * 2)) in P2; lia.
+            -- apply Z.gt_lt in P2.
+               rewrite Z.lt_le_pred in P2; simpl in P2.
+               apply (Z.mul_le_mono_nonneg_r _ _ (Z.of_nat size * 2)) in P2; lia.
+        + fin_dep_destruct y; auto; unfold Spec.getHead; simpl; destruct weq; unfold listInSpec.
+          * rewrite e, Z.sub_diag, Zmod_0_l, firstn_O; reflexivity.
+          * destruct lt_dec.
+            -- simpl in Hbound.
+               specialize (wordBound _ x10) as P1.
+               specialize (wordBound _ x6) as P2.
+               rewrite boundProofZIff in *.
+               cbn [getBool negb].
+               assert (x10 <> x6) as n' by auto; clear n.
+               apply neq_wordVal in n'.
+               specialize (hdCorrect x19 P1 P2 Hbound pow2 n') as P3.
+               rewrite hd_error_Some in P3.
+               unfold lgSize in *.
+               erewrite <- rew_swap; simpl; eauto.
+               destruct (firstn _ _); [discriminate|].
+               inv P3; simpl.
+               f_equal.
+               apply of_nat_ext.
+            -- exfalso.
+               unfold lgSize in *.
+               rewrite <- Zpow_of_nat, pow2 in *.
+               apply n0.
+               specialize (Z.mod_pos_bound
+                             (wordVal (Nat.log2_up size + 1) x6)
+                             (Z.of_nat size)
+                             ltac:(lia)) as P1; lia.
+      - hyp_consumer.
+        goal_consumer2.
+      - hyp_consumer.
+        goal_consumer1.
+        + apply functional_extensionality_dep.
+          intros; fin_dep_destruct x.
+          * simpl.
+            destruct weq; subst; simpl; symmetry; unfold listInSpec.
+            -- rewrite Z.sub_diag, Zmod_0_l, firstn_O; reflexivity.
+            -- rewrite negb_true_iff.
+               rewrite emptyb_false_len, firstn_length_le;
+                 [|simpl in *; rewrite rotateLength, <- list_arr_length; lia].
+               specialize (Nat.le_0_l
+                             (Z.to_nat ((wordVal (lgSize + 1) x19
+                                         - wordVal (lgSize + 1) x13)
+                                          mod 2 ^ Z.of_nat (lgSize + 1))))
+                 as P1.
+               destruct (le_lt_or_eq _ _ P1); auto.
+               exfalso.
+               apply neq_wordVal in n; apply n.
+               specialize (wordBound _ x13) as P2; specialize (wordBound _ x19) as P3.
+               rewrite boundProofZIff in *.
+               simpl in Hbound.
+               symmetry in H1.
+               assert (0 = Z.to_nat 0) as TMP by lia; rewrite TMP in H1; clear TMP.
+               apply Z2Nat.inj in H1; try lia; [|apply Z.mod_pos_bound; lia].
+               apply Znumtheory.Zmod_divide_minus in H1; try lia.
+               rewrite Z.sub_0_r in H1; unfold Z.divide in H1; dest.
+               unfold lgSize in *.
+               rewrite <- Zpow_of_nat, Nat.pow_add_r, pow2, Nat2Z.inj_mul in *; simpl in *.
+               destruct (Z_dec 0 x) as [[P2 | P2] | P2]; try lia.
+               ++ apply Zlt_le_succ in P2; simpl in P2; try lia.
+                  apply (Z.mul_le_mono_nonneg_r _ _ (Z.of_nat size * 2)) in P2; lia.
+               ++ apply Z.gt_lt in P2.
+                  rewrite Z.lt_le_pred in P2; simpl in P2.
+                  apply (Z.mul_le_mono_nonneg_r _ _ (Z.of_nat size * 2)) in P2; lia.
+          * fin_dep_destruct y; auto; unfold Spec.getHead; simpl; destruct weq; simpl;
+            unfold listInSpec.
+            -- rewrite e, Z.sub_diag, Zmod_0_l, firstn_O; reflexivity.
+            -- destruct lt_dec.
+               ++ simpl in Hbound.
+                  specialize (wordBound _ x19) as P1.
+                  specialize (wordBound _ x13) as P2.
+                  rewrite boundProofZIff in *.
+                  cbn [getBool negb].
+                  assert (x19 <> x13) as n' by auto; clear n.
+                  apply neq_wordVal in n'.
+                  specialize (hdCorrect x29 P1 P2 Hbound pow2 n') as P3.
+                  rewrite hd_error_Some in P3.
+                  unfold lgSize in *.
+                  erewrite <- rew_swap; simpl; eauto.
+                  destruct (firstn _ _); [discriminate|].
+                  inv P3; simpl.
+                  f_equal.
+                  apply of_nat_ext.
+               ++ exfalso.
+                  unfold lgSize in *.
+                  rewrite <- Zpow_of_nat, pow2 in *.
+                  apply n0.
+                  specialize (Z.mod_pos_bound
+                                (wordVal (Nat.log2_up size + 1) x13)
+                                (Z.of_nat size)
+                                ltac:(lia)) as P1; lia.
+        + econstructor 1; auto; normalize_key_concl; simpl.
+          * destruct weq; simpl.
+            -- simpl in Hbound.
+               rewrite Zmod_0_l, Z.add_0_r; repeat rewrite Zminus_mod_idemp_r; auto.
+            -- simpl in Hbound.
+               rewrite Zplus_mod_idemp_l, Zplus_mod_idemp_r, Zminus_mod_idemp_r.
+               specialize (wordBound _ x13) as P1.
+               specialize (wordBound _ x19) as P2.
+               rewrite boundProofZIff in *.
+               assert (x19 <> x13) as n' by auto.
+               apply neq_wordVal in n'.
+               specialize (cutLen_pred P2 P1 Hbound pow2 n') as P3; unfold lgSize in *.
+               rewrite P3; lia.
+          * repeat f_equal.
+            specialize (wordBound _ x13) as P1.
+            specialize (wordBound _ x19) as P2.
+            rewrite boundProofZIff in *.
+            destruct weq; simpl; subst; unfold listInSpec, lgSize in *.
+            -- rewrite Z.sub_diag, Zmod_0_l, Z.add_0_r.
+               repeat rewrite Zminus_mod_idemp_r.
+               rewrite Z.sub_diag, Zmod_0_l; repeat rewrite firstn_O; reflexivity.
+            -- rewrite tailCorrect; auto.
+               rewrite Zplus_mod_idemp_l, Zplus_mod_idemp_r, Zminus_mod_idemp_r.
+               assert (x19 <> x13) as n' by auto.
+               apply neq_wordVal in n'.
+               specialize (cutLen_pred P2 P1 Hbound pow2 n') as P3; unfold lgSize in *.
+               rewrite P3, Z2Nat.inj_sub; try lia.
+               rewrite rotateList_periodic at 1.
+               unfold convertToList at 1.
+               rewrite <- list_arr_length.
+               do 2 f_equal.
+               rewrite Zmod_mod', <- Zpow_of_nat, Nat2Z.id, pow2;
+                 [| rewrite <-Zpow_of_nat, pow2; lia
+                  | apply Z.mod_pos_bound; lia].
+               dest.
+               rewrite Nat2Z.inj_add, Z.pow_add_r, <-Zpow_of_nat, pow2, Z.pow_1_r in *; try lia.
+               apply Zlt_le_succ in H7.
+               rewrite <- Z.add_1_r in H7.
+               destruct (Zle_lt_or_eq _ _ H7).
+               ++ rewrite (Z.mod_small (_ + _) _); try lia.
+                  rewrite <- (Nat2Z.id size) at 3;
+                    rewrite <- (Nat2Z.id size) at 5.
+                  repeat rewrite <- Zmod_mod'; try lia.
+                  ** rewrite Z.add_mod_idemp_l; lia.
+                  ** apply OMEGA2; [apply Z.mod_pos_bound|]; lia.
+               ++ rewrite H8, Z_mod_same_full, Nat.mod_0_l; auto.
+                  rewrite <- (Nat2Z.id size) at 3.
+                  rewrite <- Zmod_mod', Zplus_mod_idemp_l, Zmod_mod'
+                  , H8, Z.mul_comm, <- Zmod_mod', Z.mod_mul; try lia.
+                  apply OMEGA2; [apply Z.mod_pos_bound|]; lia.
+      - hyp_consumer.
+        goal_consumer2.
+      - hyp_consumer.
+        rewrite <- H0 in *.
+        + goal_consumer1.
+          * simpl.
+            destruct weq; symmetry; unfold listInSpec.
+            -- clear H27 H28.
+               rewrite Nat.ltb_ge, firstn_length_le;
+                 [|simpl in *; rewrite rotateLength, <- list_arr_length; lia].
+               destruct (Zle_lt_or_eq _ _ Hbound); simpl in *; try lia.
+               exfalso; rewrite <- e in H4; simpl in H4.
+               rewrite Zplus_mod_idemp_r, Zplus_mod_idemp_l,
+               Zminus_mod_idemp_l, Z.add_simpl_l, Z.mod_small in H4; try lia.
+               unfold lgSize in *.
+               rewrite <- Zpow_of_nat, Nat.pow_add_r, pow2, Nat2Z.inj_mul in *; simpl in *; lia.
+            -- clear H27 H28; simpl.
+               rewrite Nat.ltb_lt, firstn_length_le;
+                 [|simpl in *; rewrite rotateLength, <- list_arr_length; lia].
+               destruct (Zle_lt_or_eq _ _ Hbound); simpl in *; try lia.
+               exfalso.
+               apply neq_wordVal in n; apply n; simpl.
+               rewrite <- H4, Zplus_mod_idemp_l.
+               repeat rewrite Zplus_mod_idemp_r.
+               rewrite Zplus_minus, (wordBound _ x10); reflexivity.
+          * simpl in H17; rewrite negb_true_iff in H17.
+            destruct weq; try discriminate; clear H17.
+            apply neq_wordVal in n.
+            simpl in n.
+            specialize (wordBound _ x10) as P1.
+            specialize (wordBound _ x8) as P2.
+            rewrite boundProofZIff in *.
+            simpl in Hbound.
+            assert (((wordVal (Nat.log2_up size + 1) x10 - wordVal (Nat.log2_up size + 1) x8)
+                       mod 2 ^ Z.of_nat (Nat.log2_up size + 1))%Z <> Z.of_nat size) as P3.
+            { intro; apply n; unfold lgSize in *.
+              rewrite <- H4, Zplus_mod_idemp_l;
+                repeat rewrite Zplus_mod_idemp_r.
+              rewrite Zplus_minus, Z.mod_small; auto.
+            }
+            econstructor 1; auto; normalize_key_concl; simpl.
+            -- specialize (cutLen_succ x27 P1 P2 Hbound pow2) as P4; unfold lgSize in *.
+               rewrite Zplus_mod_idemp_l, Zplus_mod_idemp_r, Zminus_mod_idemp_l, P4; lia.
+            -- repeat f_equal.
+               unfold Spec.snocInBound, listInSpec.
+               destruct Nat.ltb eqn:G.
+               ++ rewrite Nat.ltb_lt, firstn_length_le in G;
+                    [| unfold convertToList; rewrite rotateLength, <- list_arr_length; lia].
+                  unfold lgSize in *.
+                  rewrite Zplus_mod_idemp_l, Zplus_mod_idemp_r, Zminus_mod_idemp_l.
+                  rewrite (listSnoc x27 P1 P2 Hbound pow2); auto.
+                  repeat f_equal.
+                  apply functional_extensionality; intro.
+                  apply if_bool_2.
+                  destruct eqb eqn:G0, weq; auto.
+                  ** exfalso.
+                     apply n0.
+                     rewrite eqb_eq in G0; rewrite G0, to_nat_of_nat; simpl.
+                     arithmetizeWord.
+                     destruct x10; simpl.
+                     rewrite Z2Nat.id, Zmod_mod; auto.
+                     apply Z.mod_pos_bound.
+                     rewrite <- Zpow_of_nat, pow2; lia.
+                  ** exfalso.
+                     rewrite Fin_eqb_neq in G0.
+                     apply G0.
+                     arithmetizeWord; destruct x10; simpl in *.
+                     rewrite <- Zpow_of_nat, <- mod_Zmod, <- (Z2Nat.id (wordVal mod _)) in H4
+                     ; try lia.
+                     apply Nat2Z.inj in H4.
+                     rewrite Zmod_mod', Nat2Z.id in H4; try lia.
+                     rewrite (Nat.mod_small (proj1_sig _)) in H4.
+                     --- apply to_nat_inj.
+                         rewrite <- H4, to_nat_of_nat; simpl.
+                         rewrite <- (Nat2Z.id (2 ^ _)), <- Zmod_mod', Zpow_of_nat; try lia.
+                     --- rewrite pow2.
+                         apply fin_to_nat_bound.
+               ++ exfalso.
+                  rewrite Nat.ltb_ge, firstn_length_le in G.
+                  ** apply P3.
+                     apply inj_le in G.
+                     rewrite Z2Nat.id in G; try lia.
+                     apply Z.le_antisymm; auto.
+                  ** unfold convertToList; rewrite rotateLength, <- list_arr_length; lia.
+        + goal_consumer1.
+          * simpl.
+            destruct weq; symmetry; unfold listInSpec.
+            -- rewrite Nat.ltb_ge, firstn_length_le;
+                 [|simpl in *; rewrite rotateLength, <- list_arr_length; lia].
+               destruct (Zle_lt_or_eq _ _ Hbound); simpl in *; try lia.
+               exfalso; rewrite <- e in H0; simpl in H0.
+               rewrite Zplus_mod_idemp_r, Zplus_mod_idemp_l,
+               Zminus_mod_idemp_l, Z.add_simpl_l, Z.mod_small in H0; try lia.
+               unfold lgSize in *.
+               rewrite <- Zpow_of_nat, Nat.pow_add_r, pow2, Nat2Z.inj_mul in *; simpl in *; lia.
+            -- rewrite Nat.ltb_lt, firstn_length_le;
+                 [|simpl in *; rewrite rotateLength, <- list_arr_length; lia].
+               destruct (Zle_lt_or_eq _ _ Hbound); simpl in *; try lia.
+               exfalso.
+               apply neq_wordVal in n; apply n; simpl.
+               rewrite <- H0, Zplus_mod_idemp_l.
+               repeat rewrite Zplus_mod_idemp_r.
+               rewrite Zplus_minus, (wordBound _ x10); reflexivity.
+          * simpl in H17; rewrite negb_false_iff in H17.
+            destruct weq; try discriminate; clear H17.
+            specialize (wordBound _ x10) as P1.
+            specialize (wordBound _ x8) as P2.
+            rewrite boundProofZIff in *.
+            simpl in Hbound.
+            assert (((wordVal (Nat.log2_up size + 1) x10 - wordVal (Nat.log2_up size + 1) x8)
+                       mod 2 ^ Z.of_nat (Nat.log2_up size + 1))%Z = Z.of_nat size) as P3.
+            { rewrite <- e; simpl.
+              unfold lgSize in *.
+              rewrite Zplus_mod_idemp_l, Zplus_mod_idemp_r, Zminus_mod_idemp_l, Z.add_simpl_l,
+              <- Zpow_of_nat, Nat.pow_add_r, Nat.pow_1_r, pow2, <- mod_Zmod, Nat.mod_small; lia.
+            }
+            econstructor 1; auto; normalize_key_concl; simpl.
+            repeat f_equal.
+            unfold Spec.snocInBound, listInSpec.
+            destruct Nat.ltb eqn:G; auto.
+            exfalso.
+            rewrite Nat.ltb_lt, firstn_length_le in G;
+              [| unfold convertToList; rewrite rotateLength, <- list_arr_length; lia].
+            unfold lgSize in *; lia.
+      - hyp_consumer.
+        + goal_consumer2.
+        + goal_consumer2; eauto.
+      - hyp_consumer.
+        goal_consumer2.
+        econstructor 1 with (enqVal := $ 0) (deqVal := $ 0); eauto.
+        + simpl; rewrite Zmod_0_l; lia.
+        + simpl; doUpdRegs_red; reflexivity.
+        + simpl; doUpdRegs_red; unfold listInSpec.
+          rewrite firstn_O; reflexivity.
+        + rewrite doUpdRegs_preserves_keys; normalize_key_concl.
+    Qed.
+
+  End SizeGT1.
+
+End Proofs3.
