Fifo/Spec.v
@@ -6,7 +6,7 @@ Section Spec.
   Context {ifcParams : Ifc.Params}.
 
   Class Params := { sizePow2 : Nat.pow 2 lgSize = size;
-                    regList : list RegInitT;
+                    (*regList : list RegInitT;*)
                   }.
 
   Context {params : Params}.
@@ -47,7 +47,8 @@ Section Spec.
 
   Local Definition deq ty: ActionT ty (Maybe k) :=
     ReadN data: nlist ty <- listName;
-    Ret (STRUCT { "valid" ::= $$(emptyb data); "data" ::= getHead _ data } : Maybe k @# ty).
+    WriteN listName: nlist ty <- Var _ (nlist ty) (tl data);
+    Ret (STRUCT { "valid" ::= $$(negb (emptyb data)); "data" ::= getHead _ data } : Maybe k @# ty).
   
   Local Definition enq ty (new: ty k): ActionT ty Bool :=
     ReadN data: nlist ty <- listName;
